Lean4Lean/TypeChecker.lean
@@ -284,6 +284,7 @@ def reduceProj (idx : Nat) (struct : Expr) (cheapRec cheapProj : Bool) : RecM (O
   let mut c ← (if cheapProj then whnfCore struct cheapRec cheapProj else whnf struct)
   if let .lit (.strVal s) := c then
     c := .strLitToConstructor s
+    c ← whnf c
   c.withApp fun mk args => do
   let .const mkC _ := mk | return none
   let env ← getEnv
@@ -633,7 +634,7 @@ def lazyDeltaReduction (tn sn : Expr) : RecM ReductionStatus := loop tn sn 1000 
 def tryStringLitExpansionCore (t s : Expr) : RecM LBool := do
   let .lit (.strVal st) := t | return .undef
   let .app sf _ := s | return .undef
-  unless sf == .const ``String.mk [] do return .undef
+  unless sf == .const ``String.ofList [] do return .undef
   toLBoolM <| isDefEqCore (.strLitToConstructor st) s
 
 def tryStringLitExpansion (t s : Expr) : RecM LBool := do
